Leansubst/Meta.lean
@@ -1,0 +1,31 @@
+import Leansubst.Defs
+
+-- Define a new tactic notation
+syntax "tac" : tactic
+
+macro_rules
+  | `(tactic| tac) => `(tactic| assumption)
+
+example (h : p) : p := by
+  tac
+
+-- You cannot prove the following theorem using `tac`
+-- example (x : α) : x = x := by
+--  tac
+
+-- Let's extend `tac`. The tactic interpreter
+-- tries all possible macro extensions for `tac` until one succeeds
+macro_rules
+  | `(tactic| tac) => `(tactic| rfl)
+
+example (x : α) : x = x := by
+  tac
+
+example (x : α) (h : p) : x = x ∧ p := by
+  apply And.intro <;> tac
+
+-- We now add a (recursive) extension
+macro_rules | `(tactic| tac) => `(tactic| apply And.intro <;> tac)
+
+example (x : α) (h : p) : x = x ∧ p := by
+  tac
